theories/TM/Code/CaseNat.v
@@ -25,11 +25,11 @@ Section CaseNat.
            end).
 
   Definition CaseNat : pTM sigNat^+ bool 1 :=
-    Move R;;
+    Move Rmove;;
     Switch (ReadChar)
           (fun o => match o with
                  | Some (inr sigNat_S) => Return (Write (inl START)) true (* S *)
-                 | Some (inr sigNat_O) => Return (Move L) false (* O *)
+                 | Some (inr sigNat_O) => Return (Move Lmove) false (* O *)
                  | _ => Return (Nop) default (* invalid input *)
                  end).
 
@@ -57,7 +57,7 @@ Section CaseNat.
       Mk_R_p (ignoreParam (fun tin tout => forall n sn : nat, tin ≃(;sn) n -> tout ≃(;pred sn) S n)).
 
     Definition Constr_S : pTM sigNat^+ unit 1 :=
-      WriteMove (inr sigNat_S) L;; Write (inl START).
+      WriteMove (inr sigNat_S) Lmove;; Write (inl START).
 
 
     Definition Constr_S_steps := 3.
@@ -83,7 +83,7 @@ Section CaseNat.
 
     Definition Constr_O : pTM sigNat^+ unit 1 := WriteValue [ sigNat_O ].
 
-    Goal Constr_O = WriteMove (inl STOP) L;; WriteMove (inr sigNat_O) L;; Write (inl START).
+    Goal Constr_O = WriteMove (inl STOP) Lmove;; WriteMove (inr sigNat_O) Lmove;; Write (inl START).
     Proof. unfold Constr_O, WriteValue, WriteString.WriteString, encode, Encode_map, map, rev, Encode_nat, encode, repeat, app. reflexivity. Qed.
     Definition Constr_O_steps := 5.
 
