theories/TM/Code/CaseSum.v
@@ -29,7 +29,7 @@ Section CaseSum.
 
 
   Definition CaseSum : pTM (sigSum sigX sigY)^+ bool 1 :=
-    Move R;; (* skip the [START] symbol *)
+    Move Rmove;; (* skip the [START] symbol *)
     Switch (ReadChar) (* read the "constructor" symbol *)
           (fun o => match o with (* Write a new [START] symbol and terminate in the corresponding label *)
                  | Some (inr sigSum_inl) => Return (Write (inl START)) true  (* inl *)
@@ -64,10 +64,10 @@ Section CaseSum.
       Mk_R_p (ignoreParam (fun tin tout => forall (y:Y) (ss:nat), tin ≃(;ss) y -> tout ≃(;pred ss) inr y)).
 
     Definition Constr_inl : pTM (sigSum sigX sigY)^+ unit 1 :=
-      WriteMove (inr sigSum_inl) L;; Write (inl START).
+      WriteMove (inr sigSum_inl) Lmove;; Write (inl START).
 
     Definition Constr_inr : pTM (sigSum sigX sigY)^+ unit 1 :=
-      WriteMove (inr sigSum_inr) L;; Write (inl START).
+      WriteMove (inr sigSum_inr) Lmove;; Write (inl START).
 
 
     Definition Constr_inl_steps := 3.
@@ -273,7 +273,7 @@ Section CaseOption.
 
   Definition Constr_None : pTM tau^+ unit 1 := WriteValue [ sigOption_None ].
 
-  Goal Constr_None = WriteMove (inl STOP) L;; WriteMove (inr sigOption_None) L;; Write (inl START).
+  Goal Constr_None = WriteMove (inl STOP) Lmove;; WriteMove (inr sigOption_None) Lmove;; Write (inl START).
   Proof. reflexivity. Qed.
     
   Definition Constr_None_steps := 5.
