theories/TM/Code/WriteValue.v
@@ -42,7 +42,7 @@ Qed.
 
 Lemma WriteString_L_local (sig : Type) (str : list sig) t :
   str <> nil ->
-  tape_local (WriteString_Fun L t str) = rev str ++ right t.
+  tape_local (WriteString_Fun Lmove t str) = rev str ++ right t.
 Proof.
   revert t. induction str as [ | s [ | s' str'] IH]; intros; cbn in *.
   - tauto.
@@ -54,15 +54,15 @@ Qed.
 Section Test.
   Let t : tape nat := midtape [3;2;1] 4 [5;6;7].
   Let str := [3;2;1].
-  Compute WriteString_Fun L t str.
+  Compute WriteString_Fun Lmove t str.
   Compute (left t).
-  Compute (left (WriteString_Fun L t str)).
+  Compute (left (WriteString_Fun Lmove t str)).
   Compute (skipn (length str - 1) (left t)).
 End Test.
 *)
 
 Lemma WriteString_L_left (sig : Type) (str : list sig) t :
-  left (WriteString_Fun L t str) = skipn (pred (length str)) (left t).
+  left (WriteString_Fun Lmove t str) = skipn (pred (length str)) (left t).
 Proof.
   revert t. induction str as [ | s [ | s' str'] IH]; intros; cbn -[skipn] in *.
   - reflexivity.
@@ -102,7 +102,7 @@ Section WriteValue.
   Variable (sig: finType) (X: Type) (cX: codable sig X).
 
   Definition WriteValue (str : list sig) : pTM sig^+ unit 1 :=
-    WriteString L (rev (inl START :: map inr str ++ [inl STOP])).
+    WriteString Lmove (rev (inl START :: map inr str ++ [inl STOP])).
 
   Definition WriteValue_size (sig:Type) (cX: codable sig X) (x : X) (s : nat) : nat := s - (S (size _ x)).
 
